swap example proven

theories/examples/swap.v
@@ -8,6 +8,7 @@ From RichWasm.named_props Require Import named_props custom_syntax.
 Require Import RichWasm.wasm.datatypes.
 From RichWasm.iris Require Import language.cwp logrel memory runtime util.
 Require Import RichWasm.syntax.
+Require Import RichWasm.iris.logrel.logrel_properties.
 
 Set Bullet Behavior "Strict Subproofs".
 
@@ -23,7 +24,7 @@ Section swap.
   Variable mem_id : N.
   Variable alloc_id : nat.
 
-  Definition swap_type : function_type :=
+  Definition swap_type : Core.function_type :=
     InnerFunT (ForallTypeT (VALTYPE (AtomR I32R) AnyRefs)
                  (ForallTypeT (VALTYPE (AtomR I32R) AnyRefs)
                     (MonoFunT [VarT 1; VarT 0] [VarT 0; VarT 1]))).
@@ -45,7 +46,7 @@ Section swap.
       ⌜alloc_spec cl⌝ ∗
       na_inv logrel_nais (ns_fun (N.of_nat alloc_id)) (N.of_nat alloc_id ↦[wf] cl).
 
-  Definition instance_import (i : nat) (ϕ : function_type) (inst : instance) : iProp Σ :=
+  Definition instance_import (i : nat) (ϕ : Core.function_type) (inst : instance) : iProp Σ :=
     ∃ j cl,
       ⌜inst.(inst_funcs) !! i = Some j⌝ ∗
       closure_interp rti sr ϕ senv_empty cl ∗
@@ -68,6 +69,27 @@ Section swap.
 
   Definition example inst : function_closure := FC_func_native inst (Tf [] []) [] body.
 
+  (* the custom sem type is parameterized by what is stored *)
+  Definition custom_sem_type (n:nat) : (leibnizO semantic_value -n> iPropO Σ) :=
+      (λne (sv:leibnizO semantic_value) , ∃ a a32, ⌜sv = SAtoms [I32A a32]⌝ ∗ ⌜a32 = Wasm_int.Int32.repr (Z.of_N a)⌝
+             ∗ mem_id↦[wms][a]serialise_i32 (Wasm_int.Int32.repr n))%I.
+
+  Lemma custom_good (n:nat) : skind_has_stype (SVALTYPE [I32R] AnyRefs) (custom_sem_type n).
+  Proof.
+    unfold skind_has_stype.
+    split.
+    - cbn. done.
+    - intros sv. iIntros "H".
+      unfold custom_sem_type.
+      iDestruct "H" as "(%a & %a32 & -> & rest)".
+      cbn.
+      iPureIntro.
+      split; repeat constructor.
+      unfold has_areps.
+      eexists; split; first done.
+      apply Forall2_cons; split; try constructor.
+  Qed.
+
   Theorem example_swap_safe inst :
     instance_ok inst ⊢ closure_interp rti sr (InnerFunT (MonoFunT [] [])) senv_empty (example inst).
   Proof.
@@ -76,6 +98,303 @@ Section swap.
     iSplitR; first done.
     iSplitR; first done.
     iIntros "!> !> %%% Hvs1 Hos1 Hrt Hown Hfr Hrun".
-  Abort.
+
+    (* step 1 some things are empty *)
+    change (values_interp1 (map (type_interp rti sr) []) senv_empty os1) with
+      (values_interp rti sr senv_empty [] os1).
+    iEval (cbn) in "Hos1".
+    iDestruct "Hos1" as "(%fake_oss & -> & bigsep)".
+    iPoseProof (big_sepL2_length with "[$bigsep]") as "%hlen1".
+    destruct fake_oss; [|cbn in hlen1; inversion hlen1].
+    iEval (cbn) in "Hvs1".
+    iPoseProof (big_sepL2_length with "[$Hvs1]") as "%hlen2".
+    destruct vs1; [|cbn in hlen2; inversion hlen2].
+    clear_nils.
+    iClear "Hvs1 bigsep". clear hlen1 hlen2.
+    unfold body.
+    iEval (cbn) in "Hfr".
+
+
+    (* custom alloc *)
+    cwp_chomp 2.
+    iApply (cwp_seq with "[Hown Hrt Hfr Hrun]").
+    {
+      iDestruct "Halloc" as "(%cl & %Hgcalloc_idx & %Hgcalloc_spec & Hgcalloc)".
+      iApply fupd_cwp.
+      iMod (na_inv_acc with "Hgcalloc Hown") as "(>Hgcalloc_cl & Hown & Hclose)".
+      1, 2: done.
+      iAssert ((▷ N.of_nat alloc_id ↦[wf] cl ={⊤}=∗ na_own logrel_nais ⊤)%I)
+        with "[Hclose Hown]" as "Hclose".
+      { iIntros "Hcl". iApply "Hclose". iFrame. }
+
+      iApply (cwp_wand with "[Hgcalloc_cl Hfr Hrun]");
+        first iApply (Hgcalloc_spec with "Hgcalloc_cl Hfr Hrun").
+      1: done.
+      iIntros "!> %% H".
+      (* iSpecialize ("Hclose" with "[$]"). *)
+      iDestruct "H" as "(<- & Hgcalloc_cl & (%a & -> & mem_phys))".
+      iSpecialize ("Hclose" with "Hgcalloc_cl").
+      instantiate (1:= (λ fr' vs',
+          ∃ a,
+            ⌜vs' = [VAL_int32 (Wasm_int.int_of_Z i32m (Z.of_N a))]⌝ ∗
+            ⌜fr' = {| prelude.W.f_locs := []; prelude.W.f_inst := inst |}⌝ ∗
+            rt_token rti sr lpall θ ∗
+            mem_id↦[wms][a]serialise_i32 (Wasm_int.Int32.repr 7%nat) ∗
+            (|={⊤}=> na_own logrel_nais ⊤)
+            )%I).
+      iExists _.
+      iFrame.
+      done.
+    }
+    iIntros (f vs) "H Hfr Hrun".
+    iDestruct "H" as "(%a1 & -> & -> & Hrt & Hmem1 & Hown)".
+    iApply fupd_cwp.
+    iMod "Hown".
+    iModIntro.
+
+    (* chomp 3 in order for seq to keep the const somewhere for call 1. Custom alloc again *)
+    cwp_chomp 3.
+    iApply (cwp_seq with "[Hown Hrt Hfr Hrun]").
+    {
+      cwp_chomp 1.
+      iApply cwp_val_app.
+      {
+        change ([BI_const ?x]) with (to_consts [x]).
+        apply has_values_to_consts.
+      }
+      iDestruct "Halloc" as "(%cl & %Hgcalloc_idx & %Hgcalloc_spec & Hgcalloc)".
+      iApply fupd_cwp.
+      iMod (na_inv_acc with "Hgcalloc Hown") as "(>Hgcalloc_cl & Hown & Hclose)".
+      1, 2: done.
+      iAssert ((▷ N.of_nat alloc_id ↦[wf] cl ={⊤}=∗ na_own logrel_nais ⊤)%I)
+        with "[Hclose Hown]" as "Hclose".
+      { iIntros "Hcl". iApply "Hclose". iFrame. }
+
+      iApply (cwp_wand with "[Hgcalloc_cl Hfr Hrun]");
+        first iApply (Hgcalloc_spec with "Hgcalloc_cl Hfr Hrun").
+      1: done.
+      iIntros "!> %% H".
+      (* iSpecialize ("Hclose" with "[$]"). *)
+      iDestruct "H" as "(<- & Hgcalloc_cl & (%a & -> & mem_phys))".
+      iSpecialize ("Hclose" with "Hgcalloc_cl").
+      unfold fvs_combine.
+      change ([?x]++[?y]) with ([x;y]).
+      instantiate (1:= (λ fr' vs',
+          ∃ a,
+            ⌜vs' = [VAL_int32 (Wasm_int.Int32.repr (Z.of_N a1)); VAL_int32 (Wasm_int.int_of_Z i32m (Z.of_N a))]⌝ ∗
+            ⌜fr' = {| prelude.W.f_locs := []; prelude.W.f_inst := inst |}⌝ ∗
+            rt_token rti sr lpall θ ∗
+            mem_id↦[wms][a]serialise_i32 (Wasm_int.Int32.repr 42%nat) ∗
+            (|={⊤}=> na_own logrel_nais ⊤)
+            )%I).
+      iExists _.
+      iFrame.
+      done.
+    }
+    iIntros (f vs) "H Hfr Hrun".
+    iDestruct "H" as "(%a2 & -> & -> & Hrt & Hmem2 & Hown)".
+    iApply fupd_cwp.
+    iMod "Hown".
+    iModIntro.
+
+    (* for convenience *)
+    set (a1_32:=(Wasm_int.Int32.repr (Z.of_N a1))).
+    set (a2_32:=(Wasm_int.Int32.repr (Z.of_N a2))).
+
+    (* time for call of swap *)
+    cwp_chomp 3.
+    iApply (cwp_seq with "[-]"). {
+
+      iDestruct "Hswap" as "(%j & %cl & %Hreg_idx & Hcl & Hswap)".
+      iApply fupd_cwp.
+      iMod (na_inv_acc with "Hswap Hown") as "(Hswap_cl & Hown & Hclose)".
+      1, 2: done.
+      iAssert ((▷ N.of_nat j ↦[wf] cl ={⊤}=∗ na_own logrel_nais ⊤)%I)
+        with "[Hclose Hown]" as "Hclose".
+      { iIntros "Hcl2". iApply "Hclose". iFrame. }
+
+      (* we need to instantiate the closure_interp twice with the custom semantic value *)
+
+      unfold swap_type.
+      rewrite closure_interp_eq.
+      iEval (cbn) in "Hcl".
+      iDestruct "Hcl" as "#Hcl".
+      iSpecialize ("Hcl" $! (SVALTYPE [I32R] AnyRefs) (SVALTYPE [I32R] AnyRefs)).
+      iSpecialize ("Hcl" $! (custom_sem_type 7)).
+      iSpecialize ("Hcl" $! eq_refl).
+      iSpecialize ("Hcl" $! ltac:(by apply subskind_of_refl)).
+      iSpecialize ("Hcl" $! ltac:(by apply custom_good)).
+
+      (* nice - one more time *)
+      rewrite inner_closure_interp_eq.
+      unfold inner_closure_interp'.
+      unfold forall_type_interp.
+
+      iSpecialize ("Hcl" $! (SVALTYPE [I32R] AnyRefs) (SVALTYPE [I32R] AnyRefs) (custom_sem_type 42)
+                     eq_refl ltac:(by apply subskind_of_refl) ltac:(by apply custom_good)).
+
+      rewrite inner_closure_interp_eq.
+      unfold inner_closure_interp'.
+      unfold mono_closure_interp.
+
+      (* it's long and scary but we can do it :) *)
+      destruct cl as [ist [ts1 ts2] tlocs es | o b].
+      2: {
+        cbn.
+        iDestruct "Hcl" as "#Hcl".
+        done. (* that was silly *)
+      }
+      iDestruct "Hcl" as "(%trans1 & %trans2 & rest)".
+      cbn in trans1.
+      inversion trans1; subst; clear trans1.
+      cbn in trans2.
+      inversion trans2; subst; clear trans2.
+      iDestruct "rest" as "#Hcl".
+
+      iAssert (values_interp1 (map (type_interp rti sr) [VarT 1; VarT 0])
+                (senv_insert_type (SVALTYPE [I32R] AnyRefs) (SVALTYPE [I32R] AnyRefs) (custom_sem_type 42)
+                   ([], [], [], [(SVALTYPE [I32R] AnyRefs, (SVALTYPE [I32R] AnyRefs, (custom_sem_type 7)))]))
+                [I32A ((Wasm_int.Int32.repr (Z.of_N a1)));I32A (Wasm_int.Int32.repr (Z.of_N a2))])
+        with "[Hmem1 Hmem2]" as "Hvalues". {
+        iClear "Hcl".
+        cbn.
+        iExists [[I32A a1_32];[I32A a2_32]].
+        iSplitR; first done.
+        cbn.
+        iSplitL "Hmem1".
+        2: iSplitL; try done.
+        all: rewrite type_interp_eq; cbn.
+        all: iExists (SVALTYPE [I32R] AnyRefs); iSplitR; first done.
+        all: iSplitR.
+        1,3: iPureIntro; split; repeat constructor; try done.
+        1-2: eexists; split; first done; try constructor; done.
+        all: iFrame.
+        all: iExists _; iSplitR; first done; done.
+      }
+      (* note: os1 = [I32A a1_32; I32A a2_32] *)
+
+      iAssert ((atoms_interp [I32A a1_32; I32A a2_32] [VAL_int32 a1_32; VAL_int32 a2_32])%I)
+        with "[]" as "atom_interp_to_use". {
+        iClear "Hcl".
+        cbn.
+        done.
+      }
+      (* and with that, vs1 := [VAL_int32 a1_32; VAL_int32 a2_32] *)
+      iSpecialize ("Hcl" $! [VAL_int32 a1_32; VAL_int32 a2_32]  [I32A a1_32; I32A a2_32] θ).
+
+      iModIntro.
+      change ([?x;?y;?z]) with ([x;y]++[z]).
+      iApply (cwp_call with "[$] [$] [$] [-]"); try by (cbn; done).
+      {
+        change ([BI_const ?x; BI_const ?y]) with (to_consts [x;y]).
+        apply has_values_to_consts.
+      }
+      iModIntro.
+      iIntros "Hfr Hrun Hdup_cl".
+      iSpecialize ("Hclose" with "Hdup_cl").
+      iApply fupd_cwp.
+      iMod "Hclose". iModIntro.
+      iRename "Hclose" into "Hown".
+
+      iSpecialize ("Hcl" with "[$] [$] [$] [$] [$] [$]").
+
+      Opaque atoms_interp. Opaque values_interp1.
+      Opaque atom_interp.
+      cbn.
+      instantiate (1:= (λ (_ : frame) (vs2 : leibnizO (list value)),
+                        (∃ os2 : leibnizO (list atom), atoms_interp os2 vs2 ∗
+                           values_interp1 [type_interp rti sr (VarT 0); type_interp rti sr (VarT 1)]
+                             ([], [], [],
+                              [(SVALTYPE [I32R] AnyRefs, (SVALTYPE [I32R] AnyRefs, custom_sem_type 42));
+                               (SVALTYPE [I32R] AnyRefs, (SVALTYPE [I32R] AnyRefs, custom_sem_type 7))])
+                             os2) ∗
+                        (∃ θ' : address_map, rt_token rti sr lpall θ') ∗ na_own logrel_nais ⊤)%I).
+      cbn.
+      iApply (cwp_wand with "[Hcl]"); first iApply "Hcl".
+      iIntros (f v) "(Hatom & Hrt & Hown)".
+      iFrame "Hrt". iFrame "Hown".
+      (* almost iframeable, but need that length v = 1 which isn't hard *)
+      iDestruct "Hatom" as "(%os2 & Hoa & Hval)".
+      iAssert (⌜length v = 2⌝%I) with "[Hoa Hval]" as "%hlen". {
+        change (values_interp1 [type_interp rti sr ?x; type_interp rti sr ?y] ?s ?o) with
+          (values_interp rti sr s [x;y] o).
+        iPoseProof (values_interp_cons_l with "[$Hval]") as "(%o1 & %o2 & -> & Hval1 & Hval2)".
+        rewrite values_interp_one_eq.
+        rewrite !value_interp_eq.
+        cbn -[atoms_interp].
+        iDestruct "Hval1" as "(%sκ & %toinv & _ & (%a & %a32 & %toinv2 & _))".
+        inversion toinv; subst; clear toinv; inversion toinv2; subst; clear toinv2.
+        iDestruct "Hval2" as "(%sκ & %toinv & _ & (%a22 & %a232 & %toinv2 & _))".
+        inversion toinv; subst; clear toinv; inversion toinv2; subst; clear toinv2.
+        iPoseProof (big_sepL2_length with "[$Hoa]") as "%hlen".
+        cbn in hlen.
+        done.
+      }
+      iFrame.
+      done.
+    (* note that, ideally, you wouldn't do cwp_wand in such a basic manner. You would add one some of these length v facts
+     but oh well. *)
+
+    }
+    (* just 2 drops left! *)
+    iIntros (f v) "H Hfr Hrun".
+    iDestruct "H" as "((%os2 & Hoa & Hval) & Hrt & Hown)".
+    clear dependent a1.
+    clear dependent a2.
+
+    (* first redo a bit of the work from the length v lmao *)
+    change (values_interp1 [type_interp rti sr ?x; type_interp rti sr ?y] ?s ?o) with
+      (values_interp rti sr s [x;y] o).
+    iPoseProof (values_interp_cons_l with "[$Hval]") as "(%o1 & %o2 & -> & Hval2 & Hval1)".
+    rewrite values_interp_one_eq.
+    rewrite !value_interp_eq.
+    cbn -[atoms_interp].
+    iDestruct "Hval2" as "(%sκ & %toinv & %sksv1 & (%a2 & %a2_32 & %toinv2 & %Ha2_32 & Hmem2))".
+    inversion toinv; subst; clear toinv; inversion toinv2; subst; clear toinv2.
+    iDestruct "Hval1" as "(%sκ & %toinv & _ & (%a1 & %a1_32 & %toinv2 & %Ha1_32 & Hmem1))".
+    inversion toinv; subst; clear toinv; inversion toinv2; subst; clear toinv2.
+
+    iEval (cbn) in "Hoa".
+    iPoseProof (atoms_interp_cons_l with "Hoa") as "(%v2 & %v1 & -> & Hoa2 & Hoa1)".
+    rewrite atoms_interp_one_inv.
+    iDestruct "Hoa1" as "(%v & -> & Hoa1)".
+    Transparent atom_interp.
+    iEval (cbn) in "Hoa1"; iEval (cbn) in "Hoa2".
+    iDestruct "Hoa2" as "->"; iDestruct "Hoa1" as "->".
+
+    (* NOTE: here, you can see that the values have indeed been switched! *)
+
+    cwp_chomp 3.
+    iApply (cwp_seq with "[Hfr Hrun]"). {
+      cwp_chomp 1.
+      iApply cwp_val_app.
+      {
+        change [BI_const ?x] with (to_consts [x]).
+        apply has_values_to_consts.
+      }
+      iApply (cwp_drop with "[$] [$] [-]").
+      unfold fvs_combine.
+      iModIntro.
+      clear_nils.
+
+      now instantiate
+        (1:= (λ f' v,
+            ⌜f' = f⌝ ∗
+             ⌜v = [VAL_int32 (Wasm_int.Int32.repr (Z.of_N a2))]⌝)%I).
+    }
+    iIntros (ft v) "(-> & ->) Hfr Hrun".
+    cwp_chomp 2.
+    iApply (cwp_drop with "[$] [$] [-]").
+    iModIntro; cbn.
+    Transparent atoms_interp. Transparent atom_interp.
+    iFrame.
+    iExists [].
+    iSplitR; first (cbn; done).
+    iExists [].
+    iSplitR; first done.
+    cbn.
+    done.
+    (* note: slightly scary that nothing happened with the memories? Probably fine? *)
+  Qed.
 
 End swap.
